coq/theories/automation/AutomationLemmas.v
@@ -1,4 +1,4 @@
-(* Require Import impboot.functional.FunSyntax.
+Require Import impboot.functional.FunSyntax.
 Require Import impboot.functional.FunSemantics.
 Require Import impboot.functional.FunProperties.
 Require Import impboot.functional.FunValues.
@@ -510,7 +510,7 @@ Hint Resolve auto_word64_w2n : automation.
 
 (* cmp *)
 
-Global Instance Refinable_cmp : Refinable ImpSyntax.cmp :=
+(* Global Instance Refinable_cmp : Refinable ImpSyntax.cmp :=
 { encode cmp :=
   match cmp with
   | ImpSyntax.Equal => value_name "Equal"
